initial_states_simulation if we set initial_state{prog_main->prog_model}

stanfrontend/CStan.v
@@ -593,9 +593,11 @@ Inductive initial_state (p: program): state -> Prop :=
   | initial_state_data_intro: forall b f m0,
       let ge := Genv.globalenv p in
       Genv.init_mem p = Some m0 ->
-      Genv.find_symbol ge p.(prog_main) = Some b ->
+      (* Genv.find_symbol ge p.(prog_main) = Some b -> *)
+      Genv.find_symbol ge p.(prog_model) = Some b ->
       Genv.find_funct_ptr ge b = Some f ->
-      type_of_fundef f = Tfunction Tnil Tvoid cc_default ->
+      (* type_of_fundef f = Tfunction Tnil Tvoid cc_default -> *)
+      type_of_fundef f = Tfunction Tnil type_int32s cc_default ->
       initial_state p (Callstate f nil Kstop m0).
 
 Inductive final_state: state -> int -> Prop :=
